Veil/SMT/Quantifiers/Elimination.lean
@@ -253,7 +253,7 @@ end IteForallPushOutTheorems
 
 
 attribute [quantifierSimp] if_false_left if_false_right if_app
-attribute [quantifierSimp] and_imp not_imp and_self eq_self ne_eq implies_true false_implies
+attribute [quantifierSimp] and_imp Classical.not_imp and_self eq_self ne_eq implies_true false_implies
 attribute [quantifierSimp] and_true true_and and_false false_and or_true
   true_or or_false false_or iff_true true_iff iff_false false_iff
 
